clean up Termination file

coq/Lex.v
@@ -6,8 +6,12 @@ Section PairLT.
     Variables (A B : Type) (ltA : relation A) (ltB : relation B).
     
     Inductive pair_lex : A * B -> A * B -> Prop :=
-    | pair_fst_lt : forall x x' y y', ltA x x' -> pair_lex (x, y) (x', y')
-    | pair_snd_lt : forall x y y', ltB y y' -> pair_lex (x, y) (x, y').
+    | pair_fst_lt : 
+        forall x x' y y', 
+          ltA x x' -> pair_lex (x, y) (x', y')
+    | pair_snd_lt : 
+        forall x y y', 
+          ltB y y' -> pair_lex (x, y) (x, y').
     
     Hint Constructors pair_lex.
     
@@ -35,24 +39,37 @@ End PairLT.
 
 Section TripleLT.
     
-    Variables (A B C : Type) (ltA : relation A) (ltB : relation B) (ltC : relation C).
+    Variables (A B C : Type) 
+              (ltA : relation A) (ltB : relation B) (ltC : relation C).
     
     Inductive triple_lex : A * B * C -> A * B * C -> Prop :=
-    | triple_fst_lt : forall x x' y y' z z', ltA x x' -> triple_lex (x, y, z) (x', y', z')
-    | triple_snd_lt : forall x y y' z z', ltB y y' -> triple_lex (x, y, z) (x, y', z')
-    | triple_thd_lt : forall x y z z', ltC z z' -> triple_lex (x, y, z) (x, y, z').
+    | triple_fst_lt : 
+        forall x x' y y' z z', 
+          ltA x x' -> triple_lex (x, y, z) (x', y', z')
+    | triple_snd_lt : 
+        forall x y y' z z', 
+          ltB y y' -> triple_lex (x, y, z) (x, y', z')
+    | triple_thd_lt : 
+        forall x y z z', 
+          ltC z z' -> triple_lex (x, y, z) (x, y, z').
     
     Hint Constructors triple_lex.
     
     Lemma triple_lex_trans :
-      transitive _ ltA -> transitive _ ltB -> transitive _ ltC -> transitive _ triple_lex.
+      transitive _ ltA 
+      -> transitive _ ltB 
+      -> transitive _ ltC 
+      -> transitive _ triple_lex.
     Proof.
       intros tA tB tC [[x1 y1] z1] [[x2 y2] z2] [[x3 y3] z3] H12 H23.
       inv H12; inv H23; eauto.
     Defined.
     
     Lemma triple_lex_wf :
-      well_founded ltA -> well_founded ltB -> well_founded ltC -> well_founded triple_lex.
+      well_founded ltA 
+      -> well_founded ltB 
+      -> well_founded ltC 
+      -> well_founded triple_lex.
     Proof.
       intros wfA wfB wfC [[x y] z].
       revert y z.
